---
layout: post
title:  "Chapter 6"
date:   2015-12-23 15:56:00 +0200
---

### Exercise 6.1.1

    c₀   = λ. λ. 0
    c₂   = λ. λ. 1 (1 0)
    plus = λ. λ. λ. λ. 3 1 (2 0 1)
    fix  = λ. (λ. 1 (λ. (1 1) 0)) (λ. 1 (λ. (1 1) 0))
    foo  = (λ. (λ. 0)) (λ. 0)

### Exercise 6.1.5

1. $$removenames_{𝚪}(x) =$$ return the index of $$x$$ in $$𝚪$$---
   if there are multiples, return the index of the right-most one.

### Exercise 6.2.2

1. $$↑^2$$(`λ. λ. 1 (0 2)`) = `λ. λ. 1 (0 4)`
2. $$↑^2$$(`λ. 0 1 (λ. 0 1 2)`) = `λ. 0 3 (λ. 0 1 4)`
